\documentclass{article}
\usepackage{ifthen}
\usepackage{epsfig}
\usepackage[utf8]{inputenc}
\usepackage{xcolor}
\color{white}
\pagecolor{black}
\usepackage{newunicodechar}
  \newunicodechar{⁻}{${}^{-}$}% Superscript minus
  \newunicodechar{²}{${}^{2}$}% Superscript two
  \newunicodechar{³}{${}^{3}$}% Superscript three

\pagestyle{empty}
\begin{document}
\[ \mathbf{y} = \mathcal{A}(\mathbf{z}) = \mathbf{z},\]
\pagebreak

\[ \mathbf{A}(\mathbf{z}) = \mathbf{I},\]
\pagebreak

\[ d\mathbf{y} = \mathbf{A}(\mathbf{z}) d\mathbf{z} = d\mathbf{z}.\]
\pagebreak

\[ d\mathbf{z} = \mathbf{A}(\mathbf{z})^\top d\mathbf{y} = d\mathbf{y}.\]
\pagebreak

\[ d\mathbf{y} = \mathbf{A}(\mathbf{z}) d\mathbf{z}.\]
\pagebreak

\[ d\mathbf{z} = \mathbf{A}(\mathbf{z})^\top d\mathbf{y}.\]
\pagebreak

\[ \mathbf{y} = \mathcal{A}(\mathbf{z}) = \mathrm{relu}(\mathbf{z}),\]
\pagebreak

\[ \mathbf{A}(\mathbf{z}) = \mathrm{diag}(1-\mathrm{relu}(\mathbf{z})^2).\]
\pagebreak

\[ \mathbf{y} = \mathcal{A}(\mathbf{z}) = \mathrm{tanh}(\mathbf{z}),\]
\pagebreak

\[ \mathbf{A}(\mathbf{z}) = \mathrm{diag}(1-\mathrm{tanh}(\mathbf{z})^2).\]
\pagebreak

\[ \mathbf{y} = \mathcal{F}(\mathbf{p}, \mathbf{x}),\]
\pagebreak

$\mathbf{p}$
\pagebreak

\[ d\mathbf{y} = \mathbf{F}^\mathrm{p}d\mathbf{p} + 
 \mathbf{F}^\mathrm{x}d\mathbf{x},\]
\pagebreak

$\mathbf{F}^\mathrm{p}$
\pagebreak

$\mathcal{F}$
\pagebreak

$\mathbf{F}^\mathrm{x}$
\pagebreak

$\mathbf{x}$
\pagebreak

\[ d\mathbf{p} = [\mathbf{F}^\mathrm{p}]^\top d\mathbf{y},\]
\pagebreak

\[ d\mathbf{x} = [\mathbf{F}^\mathrm{x}]^\top d\mathbf{y},\]
\pagebreak

$\mathbf{W}$
\pagebreak

$\mathbf{b}$
\pagebreak

\[ \mathbf{b} = \mathbf{p}[:N_{\mathrm{out}}],\]
\pagebreak

\[ \mathbf{W} = \mathbf{p}[N_{\mathrm{out}}:].\mathrm{reshape}((N_{\mathrm{out}}, 
 N_{\mathrm{in}}), \mathrm{order="F"}),\]
\pagebreak

$N_{\mathrm{out}}$
\pagebreak

$N_{\mathrm{in}}$
\pagebreak

$d\mathbf{b}$
\pagebreak

$d\mathbf{W}$
\pagebreak

$d\mathbf{p}$
\pagebreak

\[ \mathbf{y} = \mathcal{F}(\mathbf{p}, \mathbf{x})
 = \mathcal{A}(\mathbf{Wx+b}),\]
\pagebreak

$\mathcal{A}$
\pagebreak

$\mathbf{Wx+b}$
\pagebreak

\[d\mathbf{y} = \mathbf{A}(\mathbf{Wx+b})[\mathbf{W}d
 \mathbf{x}+d\mathbf{Wx}+d\mathbf{b}],\]
\pagebreak

\[d\mathbf{y} = \mathbf{W}d\mathbf{x},\]
\pagebreak

\[d\mathbf{y} = d\mathbf{y} + d\mathbf{Wx},\]
\pagebreak

\[d\mathbf{y} = d\mathbf{y} + d\mathbf{b},\]
\pagebreak

\[d\mathbf{y} = \mathbf{A}(\mathbf{Wx+b})d\mathbf{y}.\]
\pagebreak

\[d\mathbf{y} = \mathbf{A}(\mathbf{Wx+b})^{\top}d\mathbf{y},\]
\pagebreak

\[d\mathbf{b} = d\mathbf{y},\]
\pagebreak

\[d\mathbf{W} = d\mathbf{yx}^{\top},\]
\pagebreak

\[d\mathbf{x} = \mathbf{W}^{\top}d\mathbf{y}.\]
\pagebreak

$d\mathbf{y}$
\pagebreak

\[d\mathbf{b} = \mathbf{A}(\mathbf{Wx+b})^{\top}d\mathbf{y}.\]
\pagebreak

\[\mathbf{y} = \mathbf{z}*\mathbf{x},\]
\pagebreak

$*$
\pagebreak

$z_{i}=0$
\pagebreak

$p$
\pagebreak

$z_{i}=1/(1-p)$
\pagebreak

$1-p$
\pagebreak

$z_{i}=1$
\pagebreak

$\mathbf{z}$
\pagebreak

\[d\mathbf{y} = \mathbf{z}*d\mathbf{x}.\]
\pagebreak

\[d\mathbf{x} = \mathbf{z}*d\mathbf{y}.\]
\pagebreak

\[\mathbf{y} = \alpha \mathbf{x} + \beta,\]
\pagebreak

$\alpha$
\pagebreak

$\beta$
\pagebreak

\[d\mathbf{y} = \alpha d\mathbf{x}.\]
\pagebreak

\[d\mathbf{x} = \alpha d\mathbf{y}.\]
\pagebreak

\end{document}
